Add lambda expression tests

Test/dafny0/MoreReads.dfy
@@ -90,3 +90,95 @@ ghost function R3(obj: object): int
 {
   100
 }
+
+// lambda expressions
+
+method Lambda0() {
+  var f :=
+    (x: int)
+    requires x < 100
+    reads if x == 202 then var u := 10/0; {} else {} // no problem, because of precondition
+    =>
+    2;
+  var g :=
+    (x: int)
+    reads if x == 202 then var u := 10/0; {} else {} // no problem, because of precondition
+    requires x < 100
+    =>
+    2;
+}
+
+method Lambda1() {
+  var p :=
+    ()
+    requires exists f: int ~> int :: f.requires(10) && f.reads(10) == {} && f(10) == 100
+    =>
+    var bb := exists f: int ~> int :: f.requires(10) && f.reads(10) == {} && f(10) == 100; // error: precondition on .reads
+    var cc := exists f: int ~> int :: f.reads(10) == {} && f.requires(10) && f(10) == 100;
+    var f: int ~> int :| f.requires(10) && f.reads(10) == {} && f(10) == 100;
+    var g: int ~> int :| g.reads(10) == {} && g.requires(10) && g(10) == 100; // error: precondition on .reads
+    f(10) + g(10);
+
+  var r0 :=
+    ()
+    requires exists f: int ~> int :: f.requires(10) && f.reads(10) == {} && f(10) == 100
+    reads
+      var bb := exists f: int ~> int :: f.requires(10) && f.reads(10) == {} && f(10) == 100; // error: precondition on .reads
+      var cc := exists f: int ~> int :: f.reads(10) == {} && f.requires(10) && f(10) == 100;
+      {}
+    =>
+    100;
+
+  var r1 :=
+    ()
+    reads
+      var bb := exists f: int ~> int :: f.requires(10) && f.reads(10) == {obj} && f(10) == 100; // error: precondition on .reads
+      var cc := exists f: int ~> int :: f.reads(10) == {obj} && f.requires(10) && f(10) == 100; // error: insufficient reads clause on .reads
+      {}
+    =>
+    100;
+
+  var r2 :=
+    ()
+    reads
+      var bb := exists f: int ~> int :: f.requires(10) && f.reads(10) == {obj} && f(10) == 100; // error: precondition on .reads
+      var cc := exists f: int ~> int :: f.reads(10) == {obj} && f.requires(10) && f(10) == 100; // error: insufficient reads clause on .reads
+      {obj}
+    =>
+    100;
+
+  var r3 :=
+    ()
+    reads
+      var bb := exists f: int ~> int :: f.requires(10) && f.reads(10) == {obj} && f(10) == 100; // error: precondition on .reads
+      var cc := exists f: int ~> int :: f.reads(10) == {obj} && f.requires(10) && f(10) == 100; // error: insufficient reads clause on .reads
+      {}
+    reads obj
+    =>
+    100;
+}
+
+// lambda expressions are not subject to enclosing reads clause
+
+class Cell {
+  var data: int
+}
+
+function LambdaInsideLambda0(cell: Cell): int
+{
+  var f := () reads cell => cell.data; // fine
+  2
+}
+
+function LambdaInsideLambda1(cell: Cell): int
+{
+  var f := () reads cell => cell.data;
+  f() // error: LambdaInsideLambda1 has insufficient reads clause for this call
+}
+
+function LambdaInsideLambda2(cell: Cell): int
+  reads cell
+{
+  var f := () reads cell => cell.data;
+  f() // fine, since LambdaInsideLambda2 is allowed to read c
+}
